Automating proofs.

src/Lang.v
@@ -1,5 +1,9 @@
 Require Coq.Strings.Ascii.
 Require Coq.Lists.List.
+Require Coq.Setoids.Setoid.
+Require Coq.Relations.Relations.
+Require Coq.Classes.Morphisms.
+Require Util.
 
 Open Scope char_scope. (* Ensure by default we are representing characters. *)
 
@@ -32,16 +36,16 @@ Section Defs.
 
   (** The language that rejects all strings. *)
 
-  Definition Null : language := fun w => False.
+  Definition Void : language := fun w => False.
 
-  (** Conversely, no word is in [Null]. *)
+  (** Conversely, no word is in [Void]. *)
 
-  Lemma null_not_in:
+  Lemma void_not_in:
     forall w,
-    ~ Null w.
+    ~ Void w.
   Proof.
     intros.
-    unfold Null; intros N.
+    unfold Void; intros N.
     contradiction.
   Qed.
 
@@ -125,6 +129,20 @@ Section Defs.
     eauto.
   Qed.
 
+  (** Auxiliary lemma that lets us use app when the string is not directly in
+      the form of [w1 ++ w2]. *)
+  Lemma app_in_eq:
+    forall (L1 L2:language) w1 w2 w3,
+    L1 w1 ->
+    L2 w2 ->
+    w3 = w1 ++ w2 ->
+    App L1 L2 w3.
+  Proof.
+    intros.
+    subst.
+    apply app_in; auto.
+  Qed.
+
   Lemma app_in_inv:
     forall (L1 L2:language) w,
     App L1 L2 w ->
@@ -132,6 +150,70 @@ Section Defs.
   Proof.
     unfold App; intros.
     assumption.
+  Qed.
+
+  Lemma app_l_char_in:
+    forall c (L:language) w,
+    L w ->
+    App (Char c) L (c :: w).
+  Proof.
+    intros.
+    apply app_in_eq with (w1:=[c]) (w2:=w).
+    + apply char_in.
+    + assumption.
+    + reflexivity.
+  Qed.
+
+  Lemma app_l_all_in:
+    forall (L:language) w1 w2,
+    L w2 ->
+    App All L (w1 ++ w2).
+  Proof.
+    intros.
+    apply app_in_eq with (w1:=w1) (w2:=w2).
+    + apply all_in.
+    + assumption.
+    + reflexivity.
+  Qed.
+
+  Lemma app_r_all_in:
+    forall (L:language) w1 w2,
+    L w1 ->
+    App L All (w1 ++ w2).
+  Proof.
+    intros.
+    apply app_in_eq with (w1:=w1) (w2:=w2).
+    + assumption.
+    + apply all_in.
+    + reflexivity.
+  Qed.
+
+  Lemma app_l_char_in_inv:
+    forall c L w,
+    App (Char c) L w ->
+    exists w', w = c:: w' /\ L w'.
+  Proof.
+    intros.
+    apply app_in_inv in H.
+    destruct H as (w1, (w2, (?, (Ha, Hb)))).
+    apply char_in_inv in Ha.
+    subst.
+    exists w2.
+    auto.
+  Qed.
+
+  Lemma app_r_char_in_inv:
+    forall c L w,
+    App L (Char c) w ->
+    exists w', w = w' ++ [c] /\ L w'.
+  Proof.
+    intros.
+    apply app_in_inv in H.
+    destruct H as (w1, (w2, (?, (Ha, Hb)))).
+    apply char_in_inv in Hb.
+    subst.
+    exists w1.
+    auto.
   Qed.
 
   (** Union on languages *)
@@ -250,6 +332,28 @@ Section Defs.
     intuition.
   Qed.
 
+  Lemma equiv_refl:
+    forall L,
+    Equiv L L.
+  Proof.
+    split; intros; tauto.
+  Qed.
+
+  (** Register [Equiv] in Coq's tactics. *)
+  Global Add Parametric Relation : language Equiv
+    reflexivity proved by equiv_refl
+    symmetry proved by equiv_sym
+    transitivity proved by equiv_trans
+    as r_equiv_setoid.
+
+  Goal forall (L1 L2:language), Equiv L1 L2 -> Equiv L2 L1.
+  Proof.
+    intros.
+    symmetry. (** We can apply symmetry in the goal. *)
+    rewrite H. (** We can rewrite H in the goal. *)
+    reflexivity. (** We can use reflexivity to conclude Equiv goals. *)
+  Qed.
+
   Lemma pow_equiv_in:
     forall L1 L2 n s,
     Equiv L1 L2 ->
@@ -305,9 +409,130 @@ Section Defs.
     assumption.
   Qed.
 
+  Lemma app_in_equiv:
+    forall L1 L2 L3 L4 w,
+    Equiv L1 L3 ->
+    Equiv L2 L4 ->
+    App L1 L2 w ->
+    App L3 L4 w.
+  Proof.
+    intros.
+    apply app_in_inv in H1.
+    destruct H1 as (w1, (w2, (?, (Ha, Hb)))).
+    subst.
+    apply app_in.
+    + apply H; assumption.
+    + apply H0. assumption.
+  Qed.
+
+  Lemma equiv_app:
+    forall L1 L2 L3 L4,
+    Equiv L1 L3 ->
+    Equiv L2 L4 ->
+    Equiv (App L1 L2) (App L3 L4).
+  Proof.
+    split; intros.
+    - eapply app_in_equiv; eauto.
+    - eapply app_in_equiv; eauto.
+      + apply equiv_sym. assumption.
+      + apply equiv_sym. assumption.
+  Qed.
+
+  Lemma union_in_equiv:
+    forall L1 L2 L3 L4 w,
+    Equiv L1 L3 ->
+    Equiv L2 L4 ->
+    Union L1 L2 w ->
+    Union L3 L4 w.
+  Proof.
+    intros.
+    destruct H1.
+    - apply H in H1.
+      apply union_in_l.
+      assumption.
+    - apply H0 in H1.
+      apply union_in_r.
+      assumption.
+  Qed.
+
+  Lemma equiv_union:
+    forall L1 L2 L3 L4,
+    Equiv L1 L3 ->
+    Equiv L2 L4 ->
+    Equiv (Union L1 L2) (Union L3 L4).
+  Proof.
+    split; intros.
+    - eapply union_in_equiv; eauto.
+    - eapply union_in_equiv; eauto.
+      + apply equiv_sym. assumption.
+      + apply equiv_sym. assumption.
+  Qed.
+
+  Section equiv_proper.
+  Import Morphisms.
+  (* Allow rewriting under App *)
+  Global Instance app_equiv_proper: Proper (Equiv ==> Equiv ==> Equiv) App.
+  Proof.
+    unfold Proper.
+    unfold respectful.
+    intros.
+    apply equiv_app; auto.
+  Qed.
+  (* Allow rewriting under Union *)
+  Global Instance union_equiv_proper: Proper (Equiv ==> Equiv ==> Equiv) Union.
+  Proof.
+    unfold Proper.
+    unfold respectful.
+    intros.
+    apply equiv_union; auto.
+  Qed.
+
+  Global Instance star_equiv_proper: Proper (Equiv ==> Equiv) Star.
+    unfold Proper.
+    unfold respectful.
+    apply star_equiv.
+  Qed.
+
+  End equiv_proper.
   (** Relate [All] with [Star Any]. *)
 
-  Lemma any_equiv_star_any:
+  Lemma app_assoc_in:
+    forall L1 L2 L3 s,
+    App (App L1 L2) L3 s ->
+    App L1 (App L2 L3) s.
+  Proof.
+    intros.
+    apply app_in_inv in H.
+    destruct H as (w1, (w2, (?, (Ha, Hb)))).
+    subst.
+    apply app_in_inv in Ha.
+    destruct Ha as (w3, (w4, (?, (Ha, Hc)))).
+    subst.
+    rewrite <- app_assoc.
+    auto using app_in.
+  Qed.
+
+  Lemma app_assoc_rw:
+    forall L1 L2 L3,
+    Equiv (App (App L1 L2) L3) (App L1 (App L2 L3)).
+  Proof.
+    split; intros;
+      apply app_in_inv in H;
+      destruct H as (w1, (w2, (?, (Ha, Hb))));
+      subst.
+    - apply app_in_inv in Ha.
+      destruct Ha as (w3, (w4, (?, (Ha, Hc)))).
+      subst.
+      rewrite <- app_assoc.
+      auto using app_in.
+    - apply app_in_inv in Hb.
+      destruct Hb as (w3, (w4, (?, (Hb, Hc)))).
+      subst.
+      rewrite app_assoc.
+      auto using app_in.
+  Qed.
+
+  Lemma star_any_spec:
     Equiv (Star Any) All.
   Proof.
     split; intros.
@@ -324,4 +549,308 @@ Section Defs.
       apply pow_cons with (w1:=[a]) (w2:=s); auto using any_in.
   Qed.
 
+  Lemma pow_char_in_inv:
+    forall c n w,
+    Pow (Char c) n w ->
+    w = Util.pow1 c n.
+  Proof.
+    induction n; intros.
+    - inversion H; subst; clear H.
+      reflexivity.
+    - inversion H; subst; clear H.
+      inversion H2; subst; clear H2.
+      apply IHn in H1.
+      subst.
+      reflexivity.
+  Qed.
+
+  Lemma pow_char_cons:
+    forall c n w,
+    Pow (Char c) n w ->
+    Pow (Char c) (S n) (c::w).
+  Proof.
+    intros.
+    apply pow_cons with (w1:=[c]) (w2:=w).
+    - assumption.
+    - apply char_in.
+    - reflexivity.
+  Qed.
+
+  Lemma pow_char_in:
+    forall c n,
+    Pow (Char c) n (Util.pow1 c n).
+  Proof.
+    induction n; intros.
+    - apply pow_nil.
+    - simpl.
+      apply pow_cons with (w1:=[c]) (w2:=Util.pow1 c n).
+      + assumption.
+      + apply char_in.
+      + reflexivity.
+  Qed.
+
+  Lemma pow_char_cons_inv:
+    forall c n w,
+    Pow (Char c) (S n) w ->
+    exists w', w = c::w' /\ Pow (Char c) n w'.
+  Proof.
+    intros.
+    inversion H; subst; clear H.
+    inversion H2; subst; clear H2.
+    exists w2.
+    auto.
+  Qed.
+
+  Lemma pow_pow_in_inv:
+    forall c1 c2 n1 n2 w,
+    App (Pow (Char c1) n1) (Pow (Char c2) n2) w ->
+    w = Util.pow1 c1 n1 ++ Util.pow1 c2 n2.
+  Proof.
+    intros.
+    apply app_in_inv in H.
+    destruct H as (w1, (w2, (?, (Ha, Hb)))).
+    subst.
+    apply pow_char_in_inv in Ha.
+    apply pow_char_in_inv in Hb.
+    subst.
+    reflexivity.
+  Qed.
+
+  Lemma pow_pow_in_inv_eq:
+    forall c1 c2 n1 n2 m1 m2,
+    c1 <> c2 ->
+    App (Pow (Char c1) n1) (Pow (Char c2) n2) (Util.pow1 c1 m1 ++ Util.pow1 c2 m2) ->
+    n1 = m1 /\ n2 = m2.
+  Proof.
+    intros.
+    apply pow_pow_in_inv in H0.
+    assert (n1 = m1) by eauto using Util.pow1_app_inv_eq_1.
+    subst.
+    assert (n2 = m2) by eauto using Util.pow1_app_inv_eq_2.
+    subst.
+    intuition.
+  Qed.
 End Defs.
+
+Declare Scope lang_scope.
+
+Module LangNotations.
+  Import Ascii.
+  Notation "{}" := Void : lang_scope.
+  Notation "[]" := Nil : lang_scope.
+  Infix "++" := App (right associativity, at level 60) : lang_scope.
+  Notation "a || b" := (Union a b) (at level 50, left associativity)  : lang_scope.
+  Notation "x '*'" := (Star x) (at level 20) : lang_scope.
+  Infix "^^" := Pow (right associativity, at level 20) : lang_scope.
+  Infix "==" := Equiv (left associativity, at level 40) : lang_scope.
+  Coercion Char: ascii >-> language.
+End LangNotations.
+
+Module Examples.
+  Import Ascii.
+  Import List.
+  Import LangNotations.
+  Import ListNotations.
+  Import Util.
+  Open Scope lang_scope.
+  Open Scope char_scope. (* Ensure by default we are representing characters. *)
+
+  (** Any string that ends with "a" *)
+  Definition L1 : language := All ++ "a".
+
+  (** Show that the notation above is equivalent to writing a more direct, yet
+     more verbose notation: *)
+  Lemma l1_spec:
+    L1 == fun w => exists w', (w = w' ++ ["a"]) % list.
+  Proof.
+    unfold L1; split; intros.
+    - apply app_in_inv in H.
+      destruct H as (w1, (w2, (Hi, (Hj, Hk)))).
+      subst.
+      exists w1.
+      apply char_in_inv in Hk.
+      subst.
+      reflexivity.
+    - destruct H as (w, ?).
+      subst.
+      apply app_in.
+      + apply all_in.
+      + apply char_in.
+  Qed.
+
+  (** Show that string "a" is in L1. *)
+  Goal L1 ["a"].
+  Proof.
+    unfold L1.
+    (*
+      When using LangNotations, [] now becomes language Nil. If you use []
+      to represent the empty list, you will get the following error:
+      
+         The term "[]" has type "word -> Prop" while it is expected to have type "list ascii".
+     
+      To work around the issue use nil to represent the empty string.
+     *)
+    apply app_in_eq with (w1:=nil) (w2:=["a"]). (* When using lists use nil to represent  *)
+    + apply all_in.
+    + apply char_in.
+    + auto.
+  Qed.
+
+  (** Show that the empty string is not in L1. *)
+  Goal ~ L1 nil.
+  Proof.
+    unfold L1; intros N.
+    apply app_in_inv in N.
+    destruct N as (w1, (w2, (H1, (H2, H3)))).
+    (* We gather that (H1) w1 ++ w2 is the empty string *) 
+    (* However, from (H3) we get that w2 is ["a"] *)
+    apply char_in_inv in H3.
+    subst.
+    (* We are not done, because we do not know what w1 is. Let us do a case
+       analysis on w1. *)
+    destruct w1.
+    + inversion H1. (* use the explosion principle, from w2 *)
+    + inversion H1. (* use the explosion principle, from w1 *)
+  Qed.
+
+  (** Show that string "bbba" is L1 *)
+
+  Goal L1 ["b"; "b"; "b"; "a"].
+  Proof.
+    unfold L1.
+    apply app_in_eq with (w1:=["b"; "b"; "b"]) (w2:=["a"]).
+    - apply all_in.
+    - apply char_in.
+    - reflexivity.
+  Qed.
+
+  Definition L2 : language := fun w => length w = 2.
+
+  (** Show that string "01" is in L2. *)
+  Goal L2 ["0"; "1"].
+  Proof.
+    unfold L2.
+    reflexivity.
+  Qed.
+
+  Definition L3 : language := "a" ++ All ++ "b".
+
+  Lemma l3_spec:
+    L3 == fun w => exists w', (["a"] ++ w' ++ ["b"] = w) % list.
+  Proof.
+    unfold L3; split; intros.
+    - apply app_l_char_in_inv in H.
+      destruct H as (w1, (?, Hw)).
+      apply app_r_char_in_inv in Hw.
+      destruct Hw as (w2, (?, _)).
+      subst.
+      simpl.
+      exists w2.
+      reflexivity.
+    - destruct H as (w, ?).
+      subst.
+      simpl.
+      apply app_l_char_in.
+      apply app_l_all_in.
+      apply char_in.
+  Qed.
+
+  (** We define the language in terms of the Pow and App combinators. *)
+
+  Definition L4 := fun w => exists n, ("a" ^^ n ++ "b" ^^ n) w.
+
+  (** We then show that this correspond to our expectation of when not using
+      combinators: *)
+  Lemma l4_spec:
+    L4 == fun x => exists n, (pow1 "a" n ++ pow1 "b" n = x) % list.
+  Proof.
+    unfold L4; split; intros.
+    - destruct H as (n, Hw).
+      exists n.
+      apply app_in_inv in Hw.
+      destruct Hw as (w1, (w2, (?, (Ha, Hb)))).
+      subst.
+      apply pow_char_in_inv in Ha.
+      apply pow_char_in_inv in Hb.
+      subst.
+      reflexivity.
+    - destruct H as (n, H).
+      subst.
+      exists n.
+      apply app_in.
+      + apply pow_char_in.
+      + apply pow_char_in.
+  Qed.
+
+  (** L4 accepts the empty string. *)
+  Goal L4 nil.
+  Proof.
+    unfold L4.
+    exists 0.
+    apply app_in_eq with (w1:=nil) (w2:=nil).
+    + apply pow_nil.
+    + apply pow_nil.
+    + reflexivity.
+  Qed.
+
+  (** L4 accepts a single a and a single b. *)
+  Goal L4 ["a"; "a"; "b"; "b"].
+  Proof.
+    exists 2.
+    apply app_in_eq with (w1:=["a"; "a"]) (w2:=["b"; "b"]).
+    + apply pow_char_cons, pow_char_cons.
+      apply pow_nil.
+    + apply pow_char_cons, pow_char_cons.
+      apply pow_nil.
+    + reflexivity.
+  Qed.
+
+  Goal ~ L4 ["a"; "b"; "b"].
+  Proof.
+    unfold L4;
+    intros N.
+    destruct N as (n, N).
+    (* Let us rearrange the string to be in terms of Util.pow1. *)
+    assert (R: ["a"; "b"; "b"] = (pow1 "a" 1 ++ pow1 "b" 2) % list) by reflexivity.
+    rewrite R in *; clear R.
+    (* Our language is: a^n b^n = a^1 b^2, thus n = 1 and n = 2
+       and we reach a contradiction. *) 
+    apply pow_pow_in_inv_eq in N.
+    - (* n = 1 and n = 2, contradiction *)
+      destruct N.
+      subst.
+      inversion H0.
+    - (* show that a = b *)
+      intros M.
+      inversion M.
+  Qed.
+
+  (** Show that this random string is not in L4 *)
+
+  Goal ~ L4 ["c"; "a"; "r"].
+  Proof.
+    unfold L4.
+    intros N.
+    destruct N as (n, H).
+    (* Since the left-hand side has a power, we can enforce that the first
+       character has to be a 'a' if n > 0. Let us do a case analysis on n. *)
+    destruct n. {
+      apply app_in_inv in H.
+      destruct H as (w1, (w2, (Hs, (Ha, Hb)))).
+      (* Any power of 0 yields an empty string, so w1 = [] and w2 = [] *) 
+      inversion Ha; subst.
+      inversion Hb; subst.
+      (* Thus "car" = "" which is a contradiction. *)
+      inversion Hs.
+    }
+    apply app_in_inv in H.
+    destruct H as (w1, (w2, (Hs, (Ha, Hb)))).
+    (* Ha is: a ^ (S n) = w, so we know that w = a :: w' *)
+    apply pow_char_cons_inv in Ha.
+    destruct Ha as (w', (?, ?)).
+    subst.
+    (* Hs now says that on the lhs starts with c and rhs starts with a,
+       contradiction. *)
+    inversion Hs.
+  Qed.
+End Examples.
